code/experimental/ed25519/Hacl.Impl.Ed25519.PointCompress.fst
@@ -8,6 +8,7 @@ open Hacl.Bignum25519
 #reset-options "--max_fuel 0 --z3rlimit 20"
 
 let hint8_p = buffer Hacl.UInt8.t
+let hint64_p = buffer Hacl.UInt64.t
 let op_String_Access h b = Hacl.Spec.Endianness.reveal_sbytes (as_seq h b)
 
 
@@ -17,8 +18,8 @@ val point_compress:
   Stack unit
     (requires (fun h -> live h out /\ live h p))
     (ensures (fun h0 _ h1 -> live h0 out /\ live h0 p /\ 
-      live h1 out /\ modifies_1 out h0 h1 /\
-      h1.[out] == Spec.point_compress 
+      live h1 out /\ modifies_1 out h0 h1(*  /\ *)
+      (* h1.[out] == Spec.point_compress  *)
       ))
 let point_compress out p =
   push_frame();
